minimal working syntax

syntax.sig
@@ -2,10 +2,9 @@ term  : Type
 form  : Type
 Funcs : Type
 Preds : Type
-V : Functor
 
-Func (f : Funcs) : "V (fun_ar f)" (term) -> term
-Pred (p : Preds) : "V (pred_ar p)" (term) -> form
+Func (f : Funcs) : "V f" (term) -> term
+Pred (p : Preds) : "V p" (term) -> form
 
 begin imp
     Fal : form
