FOL.v
@@ -1,39 +1,25 @@
 Require Export syntax.
 
+
+Notation "p ~> q" := (In_form_imp (Impl _ p q)) (at level 60).
+Notation "⊥" := (In_form_imp (Fal _)).
+Notation "¬ p" := (p ~> ⊥) (at level 60).
+
 Reserved Notation "A |- p" (at level 70).
-Inductive deduction (formula : Type) (A : list formula) : formula -> Prop :=
+Inductive nd (A : list form) : form -> Prop :=
   | ndHyp p : In p A -> A |- p
-where "A |- p" := (deduction _ A p).
+  | ndExp p : A |- In_form_imp (Fal _)  -> A |- p
+  | ndII p q : p :: A |- q -> A |- In_form_imp (Impl _ p q)
+  | ndIE p q : A |- In_form_imp (Impl _ p q) -> A |- p -> A |- q
+where "A |- p" := (nd A p).
 
-Lemma weakening (formula : Type) (A B : list formula) p : A |- p -> incl A B -> B |- p.
-Proof. induction 1; intro Hinc. apply ndHyp. now apply (Hinc p). Qed.
+Lemma weakening A B p : A |- p -> incl A B -> B |- p.
+Proof. induction 1; intro Hinc.
+  -apply ndHyp. now apply (Hinc p).
+  -apply ndExp. now apply IHnd.
+  -apply ndII. admit.
+  -apply (ndIE _ p). now apply IHnd1. now apply IHnd2.
+Admitted.
 
-Section implicative.
-  Variable formula : Type.
+Lemma double_neg A p : A |- p -> A |- In_form_imp ()
 
-  Inductive f_implicative : Type -> Type:=
-    | Bot : f_implicative formula
-    | Imp : formula -> formula -> f_implicative formula.
-  Notation "p ~> q" := (Imp p q) (at level 51, right associativity).
-  Notation "⊥" := (Bot).
-  Notation "¬ p" := (p ~> ⊥) (at level 50).
-
-  Reserved Notation "A |-I p" (at level 70).
-(*   Is it correct to mix formula and f_implicative on the right of |- ? *)
-  Inductive deduction_implicative (A : list formula) : formula + f_implicative formula -> Prop :=
-    | ndExp p  : A |-I inr ⊥ -> A |-I inr p
-    | ndII p q : p::A |- q  -> A |-I inr (p ~> q)
-    | ndIE p q : A |-I inr (p ~> q)  ->  A |-I inl p  -> A |-I inl q
-  where "A |-I p" := (deduction_implicative A p).
-
-  Lemma weakening_imp A B p : A |-I p -> incl A B -> B |-I p.
-  Proof. induction 1 as [ p nd | p q nd | p q nd_pq H1 nd_p ]; intro Hinc.
-    -now apply ndExp, IHnd.
-    -apply ndII. apply (weakening formula (p::A)). assumption.
-     intros a [Hhd | Htl]. now left. right. now apply (Hinc a).
-    -apply (ndIE _ p). now apply H1. now apply IHnd_p.
-  Qed.
-
-  Lemma double_neg A p : A |-I inr p -> A |-I ¬¬p.
-
-End implicative.
